proof of correctness of tensorcollections

Execution_resources/lemmas.v
@@ -238,6 +238,18 @@ Fixpoint sum {n : nat} (v : Vector nat n) :=
   | S n => v n + sum v (n := n)
 end.
 
+Fixpoint matrixsum {x y : nat} (v : Tensor' nat x y 1) :=
+  match x,y with
+  | S x, S y => sum (n := (S x)) (fun i => v i y 0) + matrixsum (x := S x) (y := y) v
+  | _,_ => 0
+end.
+
+Fixpoint tensorsum {x y z : nat} (v : Tensor' nat x y z) :=
+  match x,y,z with
+  | S x, S y, S z => matrixsum (x := (S x)) (y := S y) (fun i j _=> v i j z) + tensorsum (x := S x) (y := S y) (z := z) v
+  | _,_,_ => 0
+end.
+
 Proposition eqb_correct :
   forall m n, eqb m n = true -> m = n
 .
@@ -276,4 +288,39 @@ Proof.
     apply IHn in H0. rewrite H0.
     assert (v1 n = v2 n). apply H. apply le_n. rewrite H1.
     reflexivity.
+Qed.
+
+Proposition matrixsum_eq :
+  forall x y (v1 v2 : Tensor' nat x y 1),
+  (forall i j, i < x -> j < y -> v1 i j 0 = v2 i j 0) -> matrixsum v1 = matrixsum v2.
+Proof.
+  induction y.
+  - reflexivity.
+  - intros. simpl. destruct x; try reflexivity. assert (forall i j : nat, i < S x -> j < y -> v1 i j 0 = v2 i j 0).
+    intros. apply H with (j := j) in H0. apply H0. apply le_S in H1. apply H1.
+    apply IHy in H0. rewrite H0.
+    assert (sum (n := x) (fun i : nat => v1 i y 0) = sum (n := x) (fun i : nat => v2 i y 0)).
+      apply vector_sum_eq. intros. apply H. apply le_S in H1. apply H1. apply le_n.
+    rewrite H1.
+    assert (v1 x y 0 = v2 x y 0). apply H. apply le_n. apply le_n.
+    rewrite H2. reflexivity.
+Qed.
+
+Proposition tensorsum_eq :
+  forall x y z (v1 v2 : Tensor' nat x y z),
+  (forall i j k, i < x -> j < y -> k < z -> v1 i j k = v2 i j k) -> tensorsum v1 = tensorsum v2.
+Proof.
+  induction z.
+  - reflexivity.
+  - intros. simpl. destruct x,y; try reflexivity. assert (forall i j k : nat, i < S x -> j < S y -> k < z -> v1 i j k = v2 i j k).
+    intros. apply H with (j := j) (k := k) in H0. apply H0. apply H1. apply le_S in H2. apply H2.
+    apply IHz in H0. rewrite H0.
+    assert (matrixsum (x := S x) (y := y) (fun i j _: nat => v1 i j z) = matrixsum (x := S x) (y := y) (fun i j _ : nat => v2 i j z)).
+      apply matrixsum_eq. intros. apply H. apply H1. apply le_S in H2. apply H2. apply le_n.
+    rewrite H1.
+    assert (sum (n := x) (fun i : nat => v1 i y z) = sum (n := x) (fun i : nat => v2 i y z)).
+      apply vector_sum_eq. intros. apply H. apply le_S in H2. apply H2. apply le_n. apply le_n.
+    rewrite H2.
+    assert (v1 x y z = v2 x y z). apply H. apply le_n. apply le_n. apply le_n.
+    rewrite H3. reflexivity.
 Qed.
