Execution_resources/collections.v
@@ -34,3 +34,109 @@ Proof.
         intro. subst. apply Nat.lt_irrefl in H3. apply H3. rewrite H5 in H4.
         apply H4.
 Qed.
+
+Proposition tensorcollection_correct :
+  forall a x y z (v : Tensor' execution_resource x y z),
+      exists (m : Tensor' nat x y z), (forall i j k, i < x -> j < y -> k < z -> count a (thread_set' (v i j k)) (m i j k)) ->
+      count a (thread_set' (TensorCollection x y z v)) (tensorsum m)
+.
+Proof.
+  induction z.
+  - exists (fun i j k => 0). simpl. intros.
+    destruct x,y; try (apply empty). clear. induction x. apply empty. apply IHx.
+    clear. induction x. simpl. clear. induction y. apply empty. apply IHy. simpl in *. 
+    assert (forall T, zip (T := T) (buildList y (fun _ : nat => [])) = []).
+      intros. clear. induction y. reflexivity. apply IHy.
+    rewrite H in *. apply IHx.
+  - intros. assert ( exists m : Tensor' nat x y z,
+        (forall i j k : nat,
+         i < x -> j < y -> k < z -> count a (thread_set' (v i j k)) (m i j k)) ->
+        count a (thread_set' (TensorCollection x y z v)) (tensorsum m)). apply IHz.
+    destruct H as [fz H].
+    assert (Hy : exists f, (forall i j, i < x -> j < y -> count a (thread_set' (v i j z)) (f i j)) -> count a
+          (zip (buildList x (fun i : nat => zip (buildList y (fun k : nat => thread_set' (v i k z))))))
+          (matrixsum (x := x) (y := y) (fun i j _ : nat => f i j))). {
+          clear.
+          induction y.
+          - exists (fun i j => 0). intros. simpl. clear. destruct x. apply empty. induction x. apply empty. apply IHx.
+          - assert (Hx : exists f, (forall i, i < x -> count a (thread_set' (v i y z)) (f i)) ->
+              count a (zip (buildList x (fun i : nat => thread_set' (v i y z)))) (sum (n := x) f)). {
+            clear.
+            induction x.
+            - exists (fun i => 0). intros. apply empty.
+            - assert (exists f : nat -> nat, (forall i : nat, i < x -> count a (thread_set' (v i y z)) (f i))->
+              count a (zip (buildList x (fun i0 : nat => thread_set' (v i0 y z)))) (sum (n := x) f)).
+              apply IHx. destruct H as [f H].
+              assert (exists n, count a (thread_set' (v x y z)) n). apply count_exists.
+              destruct H0.
+              exists (fun i => if (eqb i x) then x0 else f i).
+              intros. simpl. apply cat_count. rewrite eqb_refl. apply H0.
+              assert (sum (n := x) (fun i : nat => if eqb i x then x0 else f i) = sum (n := x) f).
+              apply vector_sum_eq. intros. assert (eqb i x = false). apply eqb_correct_2.
+              intro. subst. apply Nat.lt_irrefl in H2. apply H2. rewrite H3. reflexivity.
+              rewrite H2. apply H. intros. assert (f i = if eqb i x then x0 else f i).
+              assert (eqb i x = false). apply eqb_correct_2.
+              intro. subst. apply Nat.lt_irrefl in H3. apply H3. rewrite H4. reflexivity.
+              rewrite H4. apply H1. apply le_S in H3. apply H3.
+          } assert (exists f : nat -> nat -> nat,
+          (forall i j : nat, i < x -> j < y -> count a (thread_set' (v i j z)) (f i j)) ->
+            count a (zip (buildList x (fun i : nat => zip (buildList y (fun k : nat => thread_set' (v i k z))))))
+          (matrixsum (x := x) (y := y) (fun i j _ : nat => f i j))). apply IHy.
+          destruct Hx as [fx Hx]. destruct H as [fy Hy].
+          exists (fun i j => if (eqb j y) then fx i else fy i j).
+          intros. apply transpose_lemma. simpl. destruct x.
+            + simpl. clear. induction y. apply empty. apply IHy.
+            + rewrite eqb_refl. apply cat_count.
+              * apply Hx. intros. assert (fx i = if eqb y y then fx i else fy i y).
+              rewrite eqb_refl. reflexivity. rewrite H1. apply H. apply H0. apply le_n.
+              * assert (matrixsum (x := S x) (y := y) (fun i j _ : nat => if eqb j y then fx i else fy i j) = matrixsum (x := S x) (y := y) (fun i j _ : nat => fy i j)).
+                  clear. apply matrixsum_eq. intros. assert (eqb j y = false). apply eqb_correct_2.
+                  intro. subst. apply Nat.lt_irrefl in H0. apply H0. rewrite H1. reflexivity.
+                  rewrite H0. clear H0. apply transpose_lemma. apply Hy.
+                  intros. assert (fy i j = if eqb j y then fx i else fy i j).
+                    assert (eqb j y = false). apply eqb_correct_2.
+                    intro. subst. apply Nat.lt_irrefl in H1. apply H1. rewrite H2. reflexivity.
+                  rewrite H2. apply H. apply H0. apply le_S in H1. apply H1.
+   }
+    destruct Hy as [fy Hy].
+    exists (fun i j k => if (eqb k z) then fy i j else fz i j k).
+    intros. assert (
+        (tensorsum (x := x) (y := y) (z := S z) (fun i j k : nat => if eqb k z then fy i j else fz i j k)) =
+        (tensorsum (x := x) (y := y) (z := z) fz) + (matrixsum (y := y) (x := x) (fun i j _ => fy i j))). {
+      clear. induction z.
+      + destruct x,y; simpl; try reflexivity. rewrite Nat.add_0_r. reflexivity.
+      + destruct x,y; try reflexivity.
+        assert (tensorsum (x := S x) (y := S y) (z := S z) (fun i j k : nat => if eqb k z then fy i j else fz i j k) =
+        tensorsum (x := S x) (y := S y) (z := z) fz + matrixsum (x := S x) (y := S y) (fun i j _ : nat => fy i j)).
+        apply IHz with (fz := fz). simpl.
+        simpl in H. symmetry. rewrite <- Nat.add_assoc. rewrite <- H.
+        symmetry. clear H. clear IHz.
+        rewrite eqb_refl.
+        assert (eqb z (S z) = false). apply eqb_correct_2.
+        intro. subst. apply n_Sn in H. apply H. rewrite H.
+        assert (tensorsum (x := S x) (y := S y) (z := z) (fun i j k : nat => if eqb k (S z) then fy i j else fz i j k) =
+          tensorsum (x := S x) (y := S y) (z := z) (fun i j k : nat => if eqb k z then fy i j else fz i j k)).
+          apply tensorsum_eq. intros.
+          assert (eqb k z = false). apply eqb_correct_2.
+          intro. subst. apply Nat.lt_irrefl in H2. apply H2. rewrite H3.
+          assert (eqb k (S z) = false). apply eqb_correct_2.
+          intro. subst. apply le_S in H2. apply Nat.lt_irrefl in H2. apply H2. rewrite H4.
+          reflexivity.
+        rewrite H0. rewrite Nat.add_comm.
+        rewrite <- Nat.add_assoc. apply Nat.add_cancel_l.
+        rewrite Nat.add_comm. reflexivity.
+   } rewrite H1. simpl.
+   assert (count a (zip (buildList x (fun i : nat =>
+            zip (buildList y (fun j : nat =>
+               zip (buildList (S z) (fun k : nat => thread_set' (v i j k))))))))
+                (tensorsum fz + matrixsum (x := x) (y := y) (fun i j _ : nat => fy i j))). {
+        apply transpose_lemma'. apply transpose_lemma. simpl. rewrite Nat.add_comm. apply cat_count.
+        + apply Hy. intros. assert (fy i j = if eqb z z then fy i j else fz i j z).
+          rewrite eqb_refl. reflexivity. rewrite H4. apply H0. apply H2. apply H3. apply le_n.
+        + apply transpose_lemma. apply transpose_lemma'. apply H.
+        intros. assert (count a (thread_set' (v i j k)) (if eqb k z then fy i j else fz i j k)).
+        apply H0. apply H2. apply H3. apply le_S in H4. apply H4.
+        assert (eqb k z = false). apply eqb_correct_2.
+        intro. subst. apply Nat.lt_irrefl in H4. apply H4. rewrite H6 in *. apply H5.
+  } apply H2.
+Qed.
